Auto/Translation/Lam2Lam.lean
@@ -1,0 +1,64 @@
+import Lean
+import Auto.Translation.LamReif
+
+namespace Auto.Lam2Lam
+open Embedding.Lam LamReif
+
+-- We're translating `Lam` to `Lam`. We call the first `Lam`
+--   the `high-level` one, and the second `Lam` the `low-level` one.
+
+def transLamSort (ref : State) : LamSort → TransM Nat Nat LamSort
+| .atom n => do
+  let (val, _) ← (lookupTyVal! n).run ref
+  return .atom (← transTypeAtom n val)
+| .base b => return .base b
+| .func arg res => .func <$> transLamSort ref arg <*> transLamSort ref res
+
+def transLamBaseTerm (ref : State) : LamBaseTerm → TransM Nat Nat LamBaseTerm
+| .eqI n => do
+  let (sort, _) ← (lookupLamILTy! n).run ref
+  return .eqI (← sort2LamILTyIdx sort)
+| .forallEI n => do
+  let (sort, _) ← (lookupLamILTy! n).run ref
+  return .forallEI (← sort2LamILTyIdx sort)
+| .existEI n => do
+  let (sort, _) ← (lookupLamILTy! n).run ref
+  return .existEI (← sort2LamILTyIdx sort)
+| b => return b
+
+def transLamTerm (ref : State) : LamTerm → TransM Nat Nat LamTerm
+| .atom n => do
+  let ((e, s), _) ← (lookupVarVal! n).run ref
+  let s' ← transLamSort ref s
+  return .atom (← transTermAtom n (e, s'))
+| .base b => .base <$> transLamBaseTerm ref b
+| .bvar n => return .bvar n
+| .lam s t => .lam <$> transLamSort ref s <*> transLamTerm ref t
+| .app s fn arg => .app <$> transLamSort ref s <*> transLamTerm ref fn <*> transLamTerm ref arg
+
+-- Collect essential chksteps and assertions from the high-level `lam`
+--   into the low-level `lam` such that the low-level `lam` proves `re`
+partial def collectProofFor (ref : State) (re : REntry) : TransM Nat Nat Unit := do
+  if let .some _ := (← getChkMap).find? re then
+    return
+  let (highLvlProof, _) ← (lookupREntryProof! re).run ref
+  match highLvlProof with
+  | .inl cs =>
+    let posCont (n : Nat) : TransM Nat Nat Nat := (do
+      let (re, _) ← (lookupRTable! n).run ref
+      collectProofFor ref re
+      lookupREntryPos! re)
+    let cs' : ChkStep ← (do
+      match cs with
+      | .nop => return .nop
+      | .wfOfCheck lctx t => return .wfOfCheck lctx (← transLamTerm ref t)
+      | .wfOfAppend ex pos => return .wfOfAppend ex (← posCont pos)
+      | .wfOfPrepend ex pos => return .wfOfPrepend ex (← posCont pos)
+      | .wfOfTopBeta pos => return .wfOfTopBeta (← posCont pos)
+      | .validOfTopBeta pos => return .validOfTopBeta (← posCont pos)
+      | .validOfImp p₁₂ p₁ => return .validOfImp (← posCont p₁₂) (← posCont p₁)
+      )
+    newChkStep cs' re
+  | .inr (e, t) => newAssertion e (← transLamTerm ref t)
+
+end Auto.Lam2Lam
